some improvements in Compiler2.v

Compiler2.v
@@ -2,7 +2,7 @@ Require Import Com.
 Require Import Big_Step.
 Require Import Star.
 Require Import Compiler.
-Require Import List.
+Require Import List String.
 Local Open Scope Z_scope.
 Local Open Scope list_scope.
 Import ListNotations.
@@ -22,25 +22,75 @@ Definition isuccs (i: instr) (n: Z): list Z :=
   end.
 
 Definition succs (P: list instr) (n: Z)  
-                 (exprf: { i: Z & (Z.le i 0) /\ (Nat.lt (Z.to_nat i) (List.length P))}): list Z :=
-  isuccs (znth (projT1 exprf) P ADD) n.
+                 (exprf: { i: Z |  (Z.le 0 i) /\ (Nat.lt (Z.to_nat i) (List.length P))}): list Z :=
+  isuccs (znth (proj1_sig exprf) P ADD) n.
 
-Fixpoint eqb_instr (i1 i2: instr): bool :=
-  match i1, i2 with
-    | JMP _, JMP _ 
-    | LOAD _, LOAD _
-    | LOADI _, LOADI _
-    | ADD, ADD
-    | STORE _, STORE _
-    | JMPLESS _, JMPLESS _
-    | JMPGE _, JMPGE _ => true
+Lemma succs_empty: forall n p, succs [] n p = [].
+Proof. intros.
+       unfold succs.
+       destruct p. cbn.
+       case_eq (Z.to_nat x); intros.
+       - simpl in *.
+         destruct a. rewrite H in *.
+         contradict H1. scrush.
+       - simpl. destruct a. cbn in *.
+         rewrite H in *.
+         contradict H1. scrush.
+Qed.
+
+Definition ascii_eqb (a b: Ascii.ascii) :=
+  match a, b with
+    | Ascii.Ascii a1 a2 a3 a4 a5 a6 a7 a8, Ascii.Ascii b1 b2 b3 b4 b5 b6 b7 b8 =>
+      Bool.eqb a1 b1 && 
+      Bool.eqb a2 b2 &&
+      Bool.eqb a3 b3 &&
+      Bool.eqb a4 b4 &&
+      Bool.eqb a5 b5 &&
+      Bool.eqb a6 b6 &&
+      Bool.eqb a7 b7 &&
+      Bool.eqb a8 b8
+  end.
+
+Lemma ascii_eqb_refl: forall a, ascii_eqb a a = true.
+Proof. intros.
+       induction a; intros.
+       simpl.
+       now repeat rewrite eqb_reflx.
+Qed.
+
+Fixpoint string_eqb (x y: string) :=
+  match x, y with
+    | ""%string, ""%string => true
+    | String a s1, String b s2 => 
+      if ascii_eqb a b then
+      string_eqb s1 s2 else false 
     | _, _ => false
   end.
+
+Lemma string_eqb_refl: forall x, string_eqb x x = true.
+Proof. intros.
+       induction x; intros.
+       - now simpl. 
+       - simpl. now rewrite ascii_eqb_refl.
+Qed.
+
+Fixpoint instr_eqb (i1 i2: instr): bool :=
+  match i1, i2 with
+    | JMP i, JMP j         => Z.eqb i j
+    | LOAD x, LOAD y       => string_eqb x y
+    | LOADI i, LOADI j     => Z.eqb i j
+    | ADD, ADD             => true
+    | STORE x, STORE y     => string_eqb x y
+    | JMPLESS i, JMPLESS j => Z.eqb i j
+    | JMPGE i, JMPGE j     => Z.eqb i j
+    | _, _                 => false
+  end.
+
 
 Fixpoint is_in (a: instr) (l: list instr) : bool :=
   match l with
     | [] => false
-    | b :: m => eqb_instr b a || is_in a m
+    | b :: m => instr_eqb b a || is_in a m
   end.
 
 Fixpoint is_in_Z (a: Z) (l: list Z) : bool :=
@@ -56,10 +106,12 @@ Fixpoint seqZ (start:Z) (len:nat) : list Z :=
   end.
 
 Definition _exists (P: list instr)
-                   (exprf: { i: Z & (Z.le i 0) /\ (Nat.lt (Z.to_nat i) (List.length P))}): list Z :=
+                   (exprf: { i: Z | (Z.le 0 i) /\ (Nat.lt (Z.to_nat i) (List.length P))}): list Z :=
   let l1   := succs P 0 exprf in
   let l2   := seqZ 0 (List.length P) in
   (List.filter ( fun a => negb (is_in_Z a l1)) l2).
+
+Section Bop_term_exec_n.
 
 Lemma exec_0: forall P c, exec_n P c 0 c.
 Proof. scrush. Qed.
@@ -69,19 +121,115 @@ Proof. unfold exec. intro n.
        induction n; intros.
        scrush.
        destruct H.
-       eapply @star_step with (y := x). easy.
-       apply IHn. easy.
+       eapply @star_step with (y := x); scrush.
+Qed.
+
+Lemma exec1_exec_n: forall P c1 c2, exec1 P c1 c2 <-> exec_n P c1 1 c2.
+Proof. scrush. Qed.
+
+Lemma exec_trans: forall P c1 c2 c3, exec P c1 c2 -> exec P c2 c3 -> exec P c1 c3.
+Proof. intros.
+       revert c3 H0.
+       induction H; intros;
+       [ scrush |
+        	Reconstr.hobvious (@H, @H1, @IHstar)
+		     (@Star.star_step)
+		     (@Compiler.exec) (** *hammer *)].
 Qed.
 
 Lemma exec_Suc: forall n P c1 c2 c3, exec P c1 c2 -> exec_n P c2 n c3 -> exec_n P c1 (S n) c3.
 Proof. Admitted.
 
-Lemma exec_exec_n: forall n P c1 c2, exec P c1 c2 -> exec_n P c1 n c2.
+Lemma exec_exec_n: forall P c1 c2, exec P c1 c2 -> exists n, exec_n P c1 n c2.
+Proof. intros.
+       induction H; intros.
+       - exists O. scrush.
+       - destruct IHstar as (n, IH).
+         exists (S n). apply exec_Suc with (c2 := y).
+         Focus 2. easy.
+         unfold exec. eapply star_step with (y0 := y).
+         easy. scrush.
+Qed.
+
+Lemma exec_equiv_exec_n: forall P c1 c2, exec P c1 c2 <-> exists n, exec_n P c1 n c2.
+Proof. intros. split.
+       intros; now eapply exec_exec_n in H.
+       intros. destruct H. now eapply exec_n_exec in H.
+Qed.
+
+
+Lemma exec_n_Nil_l: forall k c1 c2, exec_n [] c1 k c2 -> (c1 = c2 /\ k = O).
+Proof. intro k.
+       induction k; intros; scrush.
+Qed.
+
+Lemma exec_n_Nil_r: forall k c1 c2, (c1 = c2 /\ k = O) -> exec_n [] c1 k c2.
+Proof. intro k.
+       induction k; intros; scrush.
+Qed.
+
+Lemma exec_n_Nil: forall k c1 c2, exec_n [] c1 k c2 <-> (c1 = c2 /\ k = O).
+Proof. pose exec_n_Nil_l; pose exec_n_Nil_r; scrush. Qed.
+
+Lemma exec_n_step_l: forall k n n' P s s' stk stk',
+  n <> n' -> 
+  exec_n P (n, stk, s) k (n', stk', s') -> exists c, exec P (n, stk, s) c /\ exec_n P c (k - 1) (n', stk', s') /\ Nat.lt 0%nat k.
+Proof. intro k.
+       induction k; intros.
+       - cbn in *.
+         exists (n', stk', s'); scrush.
+       - cbn in *. destruct H0. exists x. split.
+         destruct H0.
+         unfold exec.
+         eapply @star_step with (z := x) in H0. 
+         scrush.
+         scrush.
+         assert ((k - 0)%nat = k) by scrush.
+         rewrite H1. split.
+         scrush.
+
+	     Reconstr.htrivial Reconstr.Empty
+		   (@Coq.Arith.PeanoNat.Nat.lt_0_succ, @Coq.Arith.PeanoNat.Nat.le_succ_l)
+		   (@Coq.Arith.PeanoNat.Nat.lt); Reconstr.scrush (** hammer *).
+Qed.
+
+Lemma exec_n_step_r: forall k n n' P s s' stk stk',
+  n <> n' -> 
+  (exists c, exec P (n, stk, s) c /\ exec_n P c (k - 1) (n', stk', s') /\ Nat.lt 0%nat k) -> exec_n P (n, stk, s) k (n', stk', s').
+Proof. intros.
+       case_eq k; intros.
+       - destruct H0, H0, H2. subst.
+         contradict H3. scrush.
+       - simpl. destruct H0, H0, H2.
+         eapply (exec_Suc) with (n := n0) (c3 := (n', stk', s')) in H0.
+         cbn in *. destruct H0.
+         exists x0. easy. 
+         assert ((S n0 - 1)%nat = n0) by scrush. subst.
+         now rewrite <- H4.
+Qed.
+
+End Bop_term_exec_n.
+
+Section CSES.
+
+Lemma exec_n_step: forall k n n' P s s' stk stk',
+  n <> n' ->
+  (exists c, exec P (n, stk, s) c /\ exec_n P c (k - 1) (n', stk', s') /\ Nat.lt 0%nat k) <-> 
+  exec_n P (n, stk, s) k (n', stk', s').
+Proof. split; intros. 
+       pose exec_n_step_r; scrush.
+       pose exec_n_step_l; scrush.
+Qed.
+
+Lemma exec1_end: forall P c1 c2, size P <= (fst (fst c1)) -> (exec P c1 c2 -> False).
 Proof. Admitted.
+
+
 
 (** go through the whole file..! *)
 
 
+End CSES.
 
 
 
